Weidenbach_Book/IsaSAT/IsaSAT_Stats_LLVM.thy
@@ -293,7 +293,6 @@ end
 
 abbreviation (input) \<open>restart_info_rel \<equiv> word64_rel \<times>\<^sub>r word64_rel \<times>\<^sub>r word64_rel \<times>\<^sub>r word64_rel \<times>\<^sub>r word64_rel\<close>
 abbreviation (input) restart_info_assn where
-
   \<open>restart_info_assn \<equiv> word64_assn \<times>\<^sub>a word64_assn \<times>\<^sub>a word64_assn \<times>\<^sub>a word64_assn \<times>\<^sub>a word64_assn\<close>
 
 lemma restart_info_params[sepref_import_param]:
@@ -311,7 +310,16 @@ lemmas [llvm_inline] =
   restart_info_init_def
   restart_info_restart_done_def
 
+abbreviation (input) \<open>schedule_info_rel \<equiv> word64_rel\<close>
+abbreviation (input) schedule_info_assn where
+  \<open>schedule_info_assn \<equiv> word64_assn\<close>
 
+lemma schedule_info_params[sepref_import_param]:
+  "(next_inprocessing_schedule_info, next_inprocessing_schedule_info) \<in>
+    schedule_info_rel \<rightarrow> word64_rel"
+  "(schedule_next_inprocessing_info, schedule_next_inprocessing_info) \<in>
+    schedule_info_rel \<rightarrow> schedule_info_rel"
+  by (auto)
 
 sepref_register NORMAL_PHASE QUIET_PHASE DEFAULT_INIT_PHASE
 
@@ -507,16 +515,32 @@ sepref_def ema_extract_value_impl
   apply (annot_snat_const \<open>TYPE(64)\<close>)
   by sepref
 
+sepref_def schedule_next_inprocessing_info_impl
+  is \<open>RETURN o schedule_next_inprocessing_info\<close>
+  :: \<open>schedule_info_assn\<^sup>k \<rightarrow>\<^sub>a schedule_info_assn\<close>
+  unfolding schedule_next_inprocessing_info_def
+  apply (annot_snat_const \<open>TYPE(64)\<close>)
+  by sepref
+
+sepref_def next_inprocessing_schedule_info_impl
+  is \<open>RETURN o next_inprocessing_schedule_info\<close>
+  :: \<open>schedule_info_assn\<^sup>k \<rightarrow>\<^sub>a word64_assn\<close>
+  unfolding next_inprocessing_schedule_info_def
+  by sepref
+
+
+
 
 type_synonym heur_assn = \<open>(ema \<times> ema \<times> restart_info \<times> 64 word \<times>
   (phase_saver_assn \<times> 64 word \<times> phase_saver'_assn \<times> 64 word \<times> phase_saver'_assn \<times> 64 word \<times> 64 word \<times> 64 word) \<times>
-  reluctant_rel_assn \<times> 1 word \<times> phase_saver_assn)\<close>
+  reluctant_rel_assn \<times> 1 word \<times> phase_saver_assn \<times> 64 word)\<close>
 
 definition heuristic_int_assn :: \<open>restart_heuristics \<Rightarrow> heur_assn \<Rightarrow> assn\<close> where
   \<open>heuristic_int_assn = ema_assn \<times>\<^sub>a
   ema_assn \<times>\<^sub>a
   restart_info_assn \<times>\<^sub>a
-  word64_assn \<times>\<^sub>a phase_heur_assn \<times>\<^sub>a reluctant_assn \<times>\<^sub>a bool1_assn \<times>\<^sub>a phase_saver_assn\<close>
+  word64_assn \<times>\<^sub>a phase_heur_assn \<times>\<^sub>a reluctant_assn \<times>\<^sub>a bool1_assn \<times>\<^sub>a phase_saver_assn \<times>\<^sub>a
+  schedule_info_assn\<close>
 
 abbreviation heur_int_rel :: \<open>(restart_heuristics \<times> restart_heuristics) set\<close> where
   \<open>heur_int_rel \<equiv> Id\<close>
@@ -578,14 +602,19 @@ lemma set_zero_wasted_stats_set_zero_wasted_stats:
   \<in> Id \<times>\<^sub>f Id \<times>\<^sub>f heur_rel \<rightarrow>\<^sub>f \<langle>bool_rel\<rangle>nres_rel\<close> and
   get_conflict_count_since_last_restart_stats_get_conflict_count_since_last_restart_stats:
   \<open>(get_conflict_count_since_last_restart_stats, get_conflict_count_since_last_restart)
-  \<in> heur_rel \<rightarrow> word_rel\<close>
+  \<in> heur_rel \<rightarrow> word_rel\<close> and
+  schedule_next_inprocessing_stats_schedule_next_inprocessing:
+    \<open>(schedule_next_inprocessing_stats, schedule_next_inprocessing) \<in> heur_rel \<rightarrow> heur_rel\<close> and
+  next_inprocessing_schedule_next_inprocessing_schedule_stats:
+    \<open>(next_inprocessing_schedule_info_stats, next_inprocessing_schedule) \<in> heur_rel \<rightarrow> word64_rel\<close>
   by (auto simp: set_zero_wasted_def code_hider_rel_def heuristic_reluctant_tick_def
     heuristic_reluctant_enable_def heuristic_reluctant_triggered_def apfst_def map_prod_def
     heuristic_reluctant_disable_def heuristic_reluctant_triggered2_def is_fully_propagated_heur_def
     end_of_rephasing_phase_heur_def unset_fully_propagated_heur_def restart_info_restart_done_heur_def
     heuristic_reluctant_untrigger_def set_fully_propagated_heur_def wasted_of_def get_next_phase_heur_def
     slow_ema_of_def fast_ema_of_def current_restart_phase_def incr_wasted_def current_rephasing_phase_def
-    get_conflict_count_since_last_restart_def
+    get_conflict_count_since_last_restart_def next_inprocessing_schedule_def
+    schedule_next_inprocessing_def schedule_next_inprocessing_stats_def
     intro!: frefI nres_relI
     split: prod.splits)
 
@@ -668,7 +697,7 @@ sepref_def unset_fully_propagated_heur_stats_impl
   :: \<open>heuristic_int_assn\<^sup>d \<rightarrow>\<^sub>a heuristic_int_assn\<close>
   unfolding heuristic_int_assn_def unset_fully_propagated_heur_stats_def
   by sepref
- 
+
 sepref_def restart_info_restart_done_heur_stats_impl
   is \<open>RETURN o restart_info_restart_done_heur_stats\<close>
   :: \<open>heuristic_int_assn\<^sup>d \<rightarrow>\<^sub>a heuristic_int_assn\<close>
@@ -754,7 +783,26 @@ sepref_def get_conflict_count_since_last_restart_stats_impl
   :: \<open>heuristic_int_assn\<^sup>k \<rightarrow>\<^sub>a word64_assn\<close>
   unfolding get_conflict_count_since_last_restart_stats_alt_def heuristic_int_assn_def
   by sepref
-  
+
+lemma next_inprocessing_schedule_info_stats_alt_def:
+  \<open>next_inprocessing_schedule_info_stats =
+  (\<lambda>(fast_ema, slow_ema, _, wasted, \<phi>, _,_,lits, (inprocess_schedule)). inprocess_schedule)\<close>
+  unfolding next_inprocessing_schedule_info_stats_def next_inprocessing_schedule_info_def
+  by auto
+
+sepref_def next_inprocessing_schedule_info_stats_impl
+  is \<open>RETURN o next_inprocessing_schedule_info_stats\<close>
+  :: \<open>heuristic_int_assn\<^sup>k \<rightarrow>\<^sub>a word64_assn\<close>
+  unfolding next_inprocessing_schedule_info_stats_alt_def heuristic_int_assn_def
+  by sepref
+
+sepref_def schedule_next_inprocessing_stats_impl
+  is \<open>RETURN o schedule_next_inprocessing_stats\<close>
+  :: \<open>heuristic_int_assn\<^sup>d \<rightarrow>\<^sub>a heuristic_int_assn\<close>
+  unfolding schedule_next_inprocessing_stats_def heuristic_int_assn_def
+  by sepref
+
+
 lemma hn_id_pure:
   \<open>CONSTRAINT is_pure A \<Longrightarrow> (Mreturn, RETURN o id) \<in> A\<^sup>k \<rightarrow>\<^sub>a A\<close>
   apply sepref_to_hoare
@@ -784,6 +832,8 @@ lemmas heur_refine[sepref_fr_rules] =
   current_rephasing_phase_stats_impl.refine[FCOMP current_rephasing_phase_stats_current_rephasing_phase]
   get_next_phase_heur_stats_impl.refine[FCOMP get_next_phase_heur_stats_get_next_phase_heur]
   get_conflict_count_since_last_restart_stats_impl.refine[FCOMP get_conflict_count_since_last_restart_stats_get_conflict_count_since_last_restart_stats]
+  schedule_next_inprocessing_stats_impl.refine[FCOMP schedule_next_inprocessing_stats_schedule_next_inprocessing]
+  next_inprocessing_schedule_info_stats_impl.refine[FCOMP next_inprocessing_schedule_next_inprocessing_schedule_stats]
   hn_id[of heuristic_int_assn, FCOMP get_content_hnr[of heur_int_rel]]
   hn_id[of heuristic_int_assn, FCOMP Constructor_hnr[of heur_int_rel]]
 
@@ -794,8 +844,8 @@ end
 
 
 sepref_register set_zero_wasted_stats save_phase_heur_stats heuristic_reluctant_tick_stats
-  heuristic_reluctant_tick is_fully_propagated_heur_stats get_content
-
+  heuristic_reluctant_tick is_fully_propagated_heur_stats get_content next_inprocessing_schedule_info_stats
+  schedule_next_inprocessing_stats
 
 lemma mop_save_phase_heur_stats_alt_def:
   \<open>mop_save_phase_heur_stats = (\<lambda> L b (fast_ema, slow_ema, res_info, wasted, (\<phi>, target, best), rel). do {
@@ -998,9 +1048,9 @@ sepref_def mop_mark_added_heur_stats_impl
   by sepref
 
 lemma mop_is_marked_added_heur_stats_alt_def:
-\<open>mop_is_marked_added_heur_stats =(\<lambda>(fast_ema, slow_ema, res_info, wasted, \<phi>, reluctant, fully_proped, lits_st) L. do {
-   ASSERT(is_marked_added_heur_pre_stats (fast_ema, slow_ema, res_info, wasted, \<phi>, reluctant, fully_proped, lits_st) L);
-   RETURN (is_marked_added_heur_stats (fast_ema, slow_ema, res_info, wasted, \<phi>, reluctant, fully_proped, lits_st) L)
+\<open>mop_is_marked_added_heur_stats =(\<lambda>(fast_ema, slow_ema, res_info, wasted, \<phi>, reluctant, fully_proped, lits_st, schedule) L. do {
+   ASSERT(is_marked_added_heur_pre_stats (fast_ema, slow_ema, res_info, wasted, \<phi>, reluctant, fully_proped, lits_st, schedule) L);
+   RETURN (is_marked_added_heur_stats (fast_ema, slow_ema, res_info, wasted, \<phi>, reluctant, fully_proped, lits_st, schedule) L)
   })\<close>
   by (auto simp: mop_is_marked_added_heur_stats_def intro!: ext)
 
