Weidenbach_Book/IsaSAT/IsaSAT_Garbage_Collect_LLVM.thy
@@ -2,6 +2,7 @@ theory IsaSAT_Garbage_Collect_LLVM
   imports IsaSAT_Restart_Heuristics IsaSAT_Setup_LLVM
      IsaSAT_VMTF_State_LLVM IsaSAT_Rephase_State_LLVM
      IsaSAT_Arena_Sorting_LLVM
+     IsaSAT_Show_LLVM
 begin
 
 lemma length_ll[def_pat_rules]: \<open>length_ll$xs$i \<equiv> op_list_list_llen$xs$i\<close>
@@ -166,10 +167,28 @@ sepref_register isasat_GC_clauses_wl_D
 
 lemma reset_added_heur_st_alt_def:
   \<open>reset_added_heur_st S =
-  (let (heur, S) = extract_heur_wl_heur S in update_heur_wl_heur (reset_added_heur heur) S)\<close>
+      (let should_inprocess = should_inprocess_st S;
+           (heur, S) = extract_heur_wl_heur S;
+           (stats, S) = extract_stats_wl_heur S;
+           (lcount, S) = extract_lcount_wl_heur S;
+           b = current_restart_phase heur;
+           heur = if should_inprocess then (schedule_next_inprocessing (reset_added_heur heur)) else heur;
+           _ = isasat_print_progress (if should_inprocess then 105 else 103) b stats (lcount);
+           S = update_heur_wl_heur heur (update_stats_wl_heur stats (update_lcount_wl_heur lcount S)) in
+  S)\<close>
   by (auto simp: reset_added_heur_st_def state_extractors split: isasat_int.splits
     intro!: ext)
 
+(*TODO Move*)
+sepref_register should_inprocess_st
+sepref_def should_inprocess_st
+  is \<open>RETURN o should_inprocess_st\<close>
+  :: \<open>isasat_bounded_assn\<^sup>k \<rightarrow>\<^sub>a bool1_assn\<close>
+  unfolding should_inprocess_st_def
+  by sepref
+(*END Move*)
+
+thm isasat_print_progress_stats_isasat_print_progress
 sepref_def reset_added_heur_st_impl
   is \<open>RETURN o reset_added_heur_st\<close>
   :: \<open>isasat_bounded_assn\<^sup>d \<rightarrow>\<^sub>a isasat_bounded_assn\<close>
