Weidenbach_Book/IsaSAT/IsaSAT_Restart_LLVM.thy
@@ -100,4 +100,11 @@ sepref_def isasat_fast_code
   apply (annot_snat_const \<open>TYPE(64)\<close>)
   by sepref
 
+sepref_register should_inprocess_st
+sepref_def should_inprocess_st
+  is \<open>RETURN o should_inprocess_st\<close>
+  :: \<open>isasat_bounded_assn\<^sup>k \<rightarrow>\<^sub>a bool1_assn\<close>
+  unfolding should_inprocess_st_def
+  by sepref
+
 end
